dw/DeepWeb/Free/Monad/Common.v
@@ -6,10 +6,9 @@ Set Implicit Arguments.
 Set Contextual Implicit.
 Generalizable All Variables.
 
-Require Import List.
-Import ListNotations.
 Require Import String.
-Require Fin.
+From Custom Require Import List.
+Import ListNotations.
 
 From QuickChick Require Show.
 
@@ -22,6 +21,7 @@ Import SumNotations.
 Export Failure.
 Export Reader.
 Export Writer.
+Export NonDeterminism.
 
 Definition run {E F X} (run_ : forall Y, F Y -> M E Y)
   : M (E +' F) X -> M E X :=
@@ -32,36 +32,158 @@ Definition run {E F X} (run_ : forall Y, F Y -> M E Y)
       end
   in hom run'.
 
-Module Export Basic.
-Section NonDeterminism.
+Module Type FancyNonDeterminismSig.
 
-Inductive nondetE : Type -> Type :=
-| Or : nondetE bool.
+  (* A branching computation with [n] possible futures.
+     The constructor can be annotated with a string to help
+     debugging. *)
 
-Definition or `{nondetE -< E} {X} (k1 k2 : M E X)
-  : M E X :=
-  Vis (convert Or) (fun b : bool => if b then k1 else k2).
+  Inductive nondetE : Type -> Type :=
+  | Or : forall (n : nat), string -> nondetE (Fin.t n).
+  (* BCP: What does the Fin.t do (why not just return nat)?  Where do
+     we use it? (Answer: It simplifies some proofs.  Let's leave it
+     and just explain what it means.) *)
 
-(* This can fail if the list is empty. *)
-Definition choose `{nondetE -< E} `{failureE -< E} {X}
-  : list X -> M E X := fix choose' xs : M E X :=
-  match xs with
-  | [] => fail "choose: No choice left"
-  | x :: xs =>
-    or (Ret x) (choose' xs)
-  end.
+  (* [Or] nodes can have no children ([n = 0]).  (We use only this
+     version of [fail] in the swap server development -- the one above
+     is just an example.) *)
+  Parameter fail :
+    forall {E A} `{nondetE -< E},
+      string (* reason *) -> M E A.
 
-End NonDeterminism.
-End Basic.
+  (* Disjunction between two ITrees *)
+  Parameter or :
+    forall {E A} `{nondetE -< E},
+      M E A -> M E A -> M E A.
 
-Module NonDeterminismBis.
-  Include Effect.NonDeterminism.
-  Definition upgrade_or {E A} `{nondetE -< E}
-             (e : Basic.nondetE A) : M E A :=
-    match e with
-    | Basic.Or => or (ret true) (ret false)
+  (* Notation for disjunction between [n] ITrees, optionally annotated
+     with an explanation string. *)
+  Reserved Notation "'disj' reason ( f1 | .. | fn )"
+  (at level 0, reason at next level).
+  Reserved Notation "'disj' ( f1 | .. | fn )"
+  (at level 0).
+
+  (* ITree that nondeterministically chooses an element from a list
+     and returns it. *)
+  Parameter choose :
+    forall {E A} `{nondetE -< E},
+      string (* reason *) -> list A -> M E A.
+
+  (* ITree that nondeterministically removes one element from a list
+     and returns it with the rest of the list. *)
+  Parameter pick_one :
+    forall {E A} `{nondetE -< E},
+      string -> list A -> M E (A * list A).
+
+  (* BCP: The un-similarity of names between [choose] and [pick-one]
+     is unfortunate!  (Rename pick_one to choose_) *)
+End FancyNonDeterminismSig.
+
+Module FancyNonDeterminism <: FancyNonDeterminismSig.
+  Import List.
+
+  (* Nodes can be of any arity. They are annotated with
+     a string to help debugging. *)
+  Inductive nondetE : Type -> Type :=
+  | Or : forall (n : nat), string -> nondetE (Fin.t n).
+
+  Arguments Or n reason : clear implicits.
+
+  (* [Or] nodes can have no children ([n = 0]), like [failureE]. *)
+  Definition fail {E A} `{nondetE -< E}
+             (reason : string) : M E A :=
+    Vis (convert (Or 0 reason))
+        (fun f => match f : Fin.t 0 with end).
+
+  Fixpoint ix {A} (xs : list A) (i : Fin.t (List.length xs)) : A.
+  Proof.
+    destruct xs as [| x xs']; inversion i as [ | ? i' ].
+    - apply x.
+    - apply (ix _ xs' i').
+  Defined.
+
+  (* Choose one element in a list. *)
+  Definition choose {E A} `{nondetE -< E}
+             (reason : string) (xs : list A) : M E A :=
+    Vis (convert (Or (List.length xs) reason))
+        (fun i => Ret (ix xs i)).
+
+  Definition noFinZ {A} (m : Fin.t O) : A := match m with end.
+
+  (* Extend a continuation indexed by [Fin.t] with a new case. *)
+  Definition or_ {E A n} (f1 : M E A) (f2 : Fin.t n -> M E A)
+             (m : Fin.t (S n)) : M E A :=
+    match m in Fin.t n0 return
+          match n0 with
+          | O => False : Type
+          | S n0 => (Fin.t n0 -> Fin.t n)
+          end -> _ with
+    | Fin.F1 => fun _ => f1
+    | Fin.FS m => fun id => f2 (id m)
+    end (fun x => x).
+
+  Definition VisOr {E A n} `{nondetE -< E}
+             (reason : string) (k : Fin.t n -> M E A) :
+    M E A := Vis (convert (Or n reason)) k.
+
+  Notation "'disj' reason ( f1 | .. | fn )" :=
+    (VisOr reason (or_ f1 .. (or_ fn noFinZ) ..))
+  (at level 0, reason at next level) : nondet_scope.
+
+  Notation "'disj' ( f1 | .. | fn )" :=
+    (VisOr "" (or_ f1 .. (or_ fn noFinZ) ..))
+  (at level 0) : nondet_scope.
+
+  Delimit Scope nondet_scope with nondet.
+  Open Scope nondet_scope.
+
+  Example ex_disj : M nondetE nat :=
+    (disj "test" ( ret 0 | ret 1 | ret 2 )).
+
+  Definition or {E A} `{nondetE -< E} (t1 t2 : M E A) : M E A :=
+    disj ( t1 | t2 ).
+
+  (* Remove an element from a list, also returning the remaining
+     elements. *)
+
+  (* [picks] embedded in a tree. *)
+  Definition pick_one {E A} `{nondetE -< E}
+             (reason : string) (xs : list A) : M E (A * list A) :=
+    choose reason (picks xs).
+
+  (* A few helpers for [Fin.t]. *)
+
+  (* A list of [Fin.t]. *)
+  Definition every_fin (m : nat) : list (Fin.t m) :=
+    (fix every_fin m n :=
+       match n return (Fin.t n -> Fin.t m) -> list (Fin.t m) with
+       | O => fun _ => []
+       | S n' => fun k =>
+         k (@Fin.F1 n') :: every_fin m n' (fun i => k (Fin.FS i))
+       end) m m (fun i => i).
+
+  (* Convert a [nat] to a [Fin.t] without too much care. *)
+  Fixpoint to_fin {n : nat} (m : nat) : option (Fin.t n) :=
+    match n, m return option (Fin.t n) with
+    | O, _ => None
+    | S n, O => Some Fin.F1
+    | S n, S m => option_map Fin.FS (to_fin m)
     end.
-End NonDeterminismBis.
+
+  (* Convert a [nat] to a [Fin.t] with even less care. *)
+  Fixpoint to_fin' {n : nat} (m : nat) : Fin.t (S n) :=
+    match n, m return Fin.t (S n) with
+    | O, _ => Fin.F1
+    | S n, O => Fin.F1
+    | S n, S m => Fin.FS (to_fin' m)
+    end.
+
+  Definition upgrade_or {E A} `{nondetE -< E}
+             (e : NonDeterminism.nondetE A) : M E A :=
+    match e with
+    | NonDeterminism.Or => or (ret true) (ret false)
+    end.
+End FancyNonDeterminism.
 
 Module Export State.
 Include Effect.State.
