dw/DeepWeb/Free/Monad/Effect.v
@@ -1,4 +1,4 @@
-Generalizable Variables A B C D E F.
+Generalizable Variables E.
 
 Require Import List.
 Import ListNotations.
@@ -6,119 +6,50 @@ Require Import String.
 Require Fin.
 
 From QuickChick Require Show.
+From Custom Require Import List.
 
 Require Import DeepWeb.Free.Monad.Free.
 Require Import DeepWeb.Free.Monad.Internal.
-Import MonadNotations.
+Require Export DeepWeb.Free.Monad.OpenUnion.
+Import MonadNotations SumNotations.
 
-Section Extensible.
+(* Effect types can be combined using the [+'] operator:
+   [E +' F] is the disjoint union of effects [E] and [F].
 
-(** * Combinators for Extensible Event Types *)
+   We have a typeclass [-<] ("convertible") such that
+   there is an instance of [E -< S] if [S] is a sum
+   constructed using [+'] and one of the operands is [E].
+   For example, the following instances are available:
 
-(* BCP: Move all the Convertible stuff to another file.  At the top of
-   this file, but just an informal comment explaining +' and -< *)
+   [E -< E]
+   [E -< (F +' E)]
+   [E -< (E +' F)]
+   [E -< (E +' F +' G)]
 
-(* Union of two effect types. *)
-Definition sum1 (E1 E2 : Type -> Type) (X : Type) : Type :=
-  E1 X + E2 X.
+   If [E -< S], the function [convert] injects an effect [E]
+   into the sum [S]:
 
-(* Empty effect type. *)
-Inductive emptyE : Type -> Type := .
+   [convert : E X -> S X]
 
-(* Automatic application of commutativity and associativity for sums.
+   The function [embed] further wraps an effect as a tree:
 
-   TODO: This is still quite fragile and prone to infinite instance
-   resolution loops. *)
+   [embed : E X -> M S X]
 
-Class Convertible (A B : Type -> Type) :=
-  { convert : forall {X}, A X -> B X }.
+   [embed] can also transform unapplied or partially-applied
+   constructors.
 
-(* Don't try to guess. *)
-Global Instance fluid_id A : Convertible A A | 0 :=
-  { convert X a := a }.
+   [embed : (I -> E X) -> (I -> M S X)]
+   [embed : (I -> J -> E X) -> (I -> J -> M S X)]
 
-(* Destructure sums. *)
-Global Instance fluid_sum `{Convertible A C} `{Convertible B C}
-  : Convertible (sum1 A B) C | 7 :=
-  { convert X ab :=
-      match ab with
-      | inl a => convert a
-      | inr b => convert b
-      end }.
+   Using [-<], we can write functions that are polymorphic
+   over all sums containing containing some effects.
+   For example, [fail] (defined just below) can be used in any
+   tree that includes the [failureE] effect:
 
-(* Lean left by default for no reason. *)
-Global Instance fluid_left `{Convertible A B} C
-  : Convertible A (sum1 B C) | 8 :=
-  { convert X a := inl (convert a) }.
+   [fail : forall E `{failureE -< E}, string -> M E S]
 
-(* Very incoherent instances. *)
-Global Instance fluid_right `{Convertible A C} B
-  : Convertible A (sum1 B C) | 9 :=
-  { convert X a := inr (convert a) }.
+ *)
 
-Global Instance fluid_empty A : Convertible emptyE A :=
-  { convert X v := match v with end }.
-
-End Extensible.
-
-Notation "E1 +' E2" := (sum1 E1 E2)
-(at level 50, left associativity) : type_scope.
-
-Notation "E ++' EE" := (List.fold_left sum1 EE E)
-(at level 50, left associativity) : type_scope.
-
-Notation "E -< F" := (Convertible E F)
-(at level 90, left associativity) : type_scope.
-
-Module Import SumNotations.
-
-(* Is this readable? *)
-(* Readable, yes.  Understandable (i.e., can I guess what it's
-   for?), not really. *)
-
-Delimit Scope sum_scope with sum.
-Bind Scope sum_scope with sum1.
-
-Notation "(| x )" := (inr x) : sum_scope.
-Notation "( x |)" := (inl x) : sum_scope.
-Notation "(| x |)" := (inl (inr x)) : sum_scope.
-Notation "( x ||)" := (inl (inl x)) : sum_scope.
-Notation "(| x ||)" := (inl (inl (inr x))) : sum_scope.
-Notation "( x |||)" := (inl (inl (inl x))) : sum_scope.
-Notation "(| x |||)" := (inl (inl (inl (inr x)))) : sum_scope.
-Notation "( x ||||)" := (inl (inl (inl (inl x)))) : sum_scope.
-Notation "(| x ||||)" :=
-  (inl (inl (inl (inl (inr x))))) : sum_scope.
-Notation "( x |||||)" :=
-  (inl (inl (inl (inl (inl x))))) : sum_scope.
-Notation "(| x |||||)" :=
-  (inl (inl (inl (inl (inl (inr x)))))) : sum_scope.
-Notation "( x ||||||)" :=
-  (inl (inl (inl (inl (inl (inl x)))))) : sum_scope.
-Notation "(| x ||||||)" :=
-  (inl (inl (inl (inl (inl (inl (inr x))))))) : sum_scope.
-Notation "( x |||||||)" :=
-  (inl (inl (inl (inl (inl (inl (inl x))))))) : sum_scope.
-
-End SumNotations.
-
-Open Scope sum_scope.
-
-Definition lift {E F X} `{Convertible E F} : M E X -> M F X :=
-  hoist (@convert _ _ _).
-
-Class Embed X Y :=
-  { embed : X -> Y }.
-
-Instance Embed_fun A X Y `{Embed X Y} : Embed (A -> X) (A -> Y) :=
-  { embed := fun x a => embed (x a) }.
-
-Instance Embed_eff E F X `{Convertible E F} : Embed (E X) (M F X) :=
-  { embed := fun e => liftE (convert e) }.
-
-Arguments embed {X Y _} e.
-
-Notation "^ x" := (embed x) (at level 80).
 
 (** * Basic Effects *)
 
@@ -157,58 +88,31 @@ Arguments Put {S}.
 End State.
 
 (** ** Nondeterminism *)
+Module NonDeterminism.
+Import Failure.
 
-(* BCP: Needs some kind of introduction
+Inductive nondetE : Type -> Type :=
+| Or : nondetE bool.
 
-   We show a minimized module signature for the sake of brevity.
-   The implementation is at the end of this file. *)
+Definition or {E} `{nondetE -< E} {X} (k1 k2 : M E X)
+  : M E X :=
+  Vis (convert Or) (fun b : bool => if b then k1 else k2).
 
-Module Type NonDeterminismSig.
+(* This can fail if the list is empty. *)
+Definition choose {E} `{failureE -< E} `{nondetE -< E} {X}
+  : list X -> M E X := fix choose' xs : M E X :=
+  match xs with
+  | [] => fail "choose: No choice left"
+  | x :: xs =>
+    or (Ret x) (choose' xs)
+  end.
 
-  (* A branching computation with [n] possible futures.
-     The constructor can be annotated with a string to help
-     debugging. *)
+Global Notation "'disj' ( x | .. | y | z )" :=
+  (or x .. (or y z) ..) : nondet_scope.
 
-  Inductive nondetE : Type -> Type :=
-  | Or : forall (n : nat), string -> nondetE (Fin.t n).
-  (* BCP: What does the Fin.t do (why not just return nat)?  Where do
-     we use it? (Answer: It simplifies some proofs.  Let's leave it
-     and just explain what it means.) *)
+Delimit Scope nondet_scope with nondet.
 
-  (* [Or] nodes can have no children ([n = 0]).  (We use only this
-     version of [fail] in the swap server development -- the one above
-     is just an example.) *)
-  Parameter fail :
-    forall {E A} `{nondetE -< E},
-      string (* reason *) -> M E A.
-
-  (* Disjunction between two ITrees *)
-  Parameter or :
-    forall {E A} `{nondetE -< E},
-      M E A -> M E A -> M E A.
-
-  (* Notation for disjunction between [n] ITrees, optionally annotated
-     with an explanation string. *)
-  Reserved Notation "'disj' reason ( f1 | .. | fn )"
-  (at level 0, reason at next level).
-  Reserved Notation "'disj' ( f1 | .. | fn )"
-  (at level 0).
-
-  (* ITree that nondeterministically chooses an element from a list
-     and returns it. *)
-  Parameter choose :
-    forall {E A} `{nondetE -< E},
-      string (* reason *) -> list A -> M E A.
-
-  (* ITree that nondeterministically removes one element from a list
-     and returns it with the rest of the list. *)
-  Parameter pick_one :
-    forall {E A} `{nondetE -< E},
-      string -> list A -> M E (A * list A).
-
-  (* BCP: The un-similarity of names between [choose] and [pick-one]
-     is unfortunate!  (Rename pick_one to choose_) *)
-End NonDeterminismSig.
+End NonDeterminism.
 
 (** ** Immutable State ([Reader]) *)
 
@@ -270,119 +174,3 @@ End Writer.
    they are interpreted: a [get] is assumed to get the value
    of the last [put], whereas [ask] is always going to return
    the same value. *)
-
-(****************************** Internals ***************************)
-
-(* Implementation of the nondeterminism signature. *)
-
-Module NonDeterminism <: NonDeterminismSig.
-  Import List.
-
-  (* Nodes can be of any arity. They are annotated with
-     a string to help debugging. *)
-  Inductive nondetE : Type -> Type :=
-  | Or : forall (n : nat), string -> nondetE (Fin.t n).
-
-  Arguments Or n reason : clear implicits.
-
-  (* [Or] nodes can have no children ([n = 0]), like [failureE]. *)
-  Definition fail {E A} `{nondetE -< E}
-             (reason : string) : M E A :=
-    Vis (convert (Or 0 reason))
-        (fun f => match f : Fin.t 0 with end).
-
-  Fixpoint ix {A} (xs : list A) (i : Fin.t (List.length xs)) : A.
-  Proof.
-    destruct xs as [| x xs']; inversion i as [ | ? i' ].
-    - apply x.
-    - apply (ix _ xs' i').
-  Defined.
-
-  (* Choose one element in a list. *)
-  Definition choose {E A} `{nondetE -< E}
-             (reason : string) (xs : list A) : M E A :=
-    Vis (convert (Or (length xs) reason)) (fun i => Ret (ix xs i)).
-
-  Definition noFinZ {A} (m : Fin.t O) : A := match m with end.
-
-  (* Extend a continuation indexed by [Fin.t] with a new case. *)
-  Definition or_ {E A n} (f1 : M E A) (f2 : Fin.t n -> M E A)
-             (m : Fin.t (S n)) : M E A :=
-    match m in Fin.t n0 return
-          match n0 with
-          | O => False : Type
-          | S n0 => (Fin.t n0 -> Fin.t n)
-          end -> _ with
-    | Fin.F1 => fun _ => f1
-    | Fin.FS m => fun id => f2 (id m)
-    end (fun x => x).
-
-  Definition VisOr {E A n} `{nondetE -< E}
-             (reason : string) (k : Fin.t n -> M E A) :
-    M E A := Vis (convert (Or n reason)) k.
-
-  Notation "'disj' reason ( f1 | .. | fn )" :=
-    (VisOr reason (or_ f1 .. (or_ fn noFinZ) ..))
-  (at level 0, reason at next level) : nondet_scope.
-
-  Notation "'disj' ( f1 | .. | fn )" :=
-    (VisOr "" (or_ f1 .. (or_ fn noFinZ) ..))
-  (at level 0) : nondet_scope.
-
-  Delimit Scope nondet_scope with nondet.
-  Open Scope nondet_scope.
-
-  Example ex_disj : M nondetE nat :=
-    (disj "test" ( ret 0 | ret 1 | ret 2 )).
-
-  Definition or {E A} `{nondetE -< E} (t1 t2 : M E A) : M E A :=
-    disj ( t1 | t2 ).
-
-  (* Remove an element from a list, also returning the remaining
-     elements. *)
-
-  (* Helper for [picks]. *)
-  Fixpoint picks' {A} (xs1 xs2 : list A) : list (A * list A) :=
-    match xs2 with
-    | [] => []
-    | x2 :: xs2' =>
-      (x2, rev_append xs1 xs2') :: picks' (x2 :: xs1) xs2'
-    end.
-
-  (* List of ways to pick an element out of a list. *)
-  Definition picks {A} (xs : list A) : list (A * list A) :=
-    picks' [] xs.
-
-  (* [picks] embedded in a tree. *)
-  Definition pick_one {E A} `{nondetE -< E}
-             (reason : string) (xs : list A) : M E (A * list A) :=
-    choose reason (picks xs).
-
-  (* A few helpers for [Fin.t]. *)
-
-  (* A list of [Fin.t]. *)
-  Definition every_fin (m : nat) : list (Fin.t m) :=
-    (fix every_fin m n :=
-       match n return (Fin.t n -> Fin.t m) -> list (Fin.t m) with
-       | O => fun _ => []
-       | S n' => fun k =>
-         k (@Fin.F1 n') :: every_fin m n' (fun i => k (Fin.FS i))
-       end) m m (fun i => i).
-
-  (* Convert a [nat] to a [Fin.t] without too much care. *)
-  Fixpoint to_fin {n : nat} (m : nat) : option (Fin.t n) :=
-    match n, m return option (Fin.t n) with
-    | O, _ => None
-    | S n, O => Some Fin.F1
-    | S n, S m => option_map Fin.FS (to_fin m)
-    end.
-
-  (* Convert a [nat] to a [Fin.t] with even less care. *)
-  Fixpoint to_fin' {n : nat} (m : nat) : Fin.t (S n) :=
-    match n, m return Fin.t (S n) with
-    | O, _ => Fin.F1
-    | S n, O => Fin.F1
-    | S n, S m => Fin.FS (to_fin' m)
-    end.
-
-End NonDeterminism.
