dw/DeepWeb/Lib/SimpleSpec.v
@@ -4,7 +4,7 @@ Import MonadNotations.
 
 Require Import DeepWeb.Free.Monad.Free.
 Require Import DeepWeb.Free.Monad.Common.
-Import NonDeterminismBis SumNotations.
+Import SumNotations.
 
 Require Import DeepWeb.Lib.Util.
 
@@ -19,81 +19,114 @@ From DeepWeb Require Export
 
 (** * Interfaces *)
 
-(** ** Network *)
+(** ** Server *)
 
-(* Types and operations for defining server ITrees.  For more details,
-   see [Lib.SimpleSpec_Server]. *)
+(* Types and operations for defining server implementation ITrees.
+   For more details, see [Lib.SimpleSpec_Server]. *)
 Module Type ServerIface.
 
 (* A server is a program with internal nondeterminism and
    external network effects. *)
-Parameter serverE : Type -> Type.
-
-(* Internal nondeterminism is implemented via [nondetE]. *)
-Declare Instance nondet_server : nondetE -< serverE.
+Inductive serverE : Type -> Type :=
 
 (* Accept a new connection. *)
-Parameter accept : M serverE connection_id.
+| Accept   : serverE connection_id
 
 (* Receive one byte from a connection. *)
-Parameter recv_byte : connection_id -> M serverE byte.
+| RecvByte : connection_id -> serverE byte
 
 (* Send one byte to a connection. *)
-Parameter send_byte : connection_id -> byte -> M serverE unit.
+| SendByte : connection_id -> byte -> serverE unit
+.
+
+(* The server monad to write implementations in.
+   A server is a program with internal nondeterminism and
+   external network effects. *)
+Definition ServerM := M (failureE +' nondetE +' serverE).
+
+(* We wrap these constructors into [ServerM] values for convenience. *)
+
+Definition accept :
+  ServerM connection_id := embed Accept.
+Definition recv_byte :
+  connection_id -> ServerM byte := embed RecvByte.
+Definition send_byte :
+  connection_id -> byte -> ServerM unit := embed SendByte.
+
+(* Here are a few more useful operations written using those
+   above. *)
 
 (* Receive up to [n] bytes, nondeterministically. *)
-Parameter recv : connection_id -> nat -> M serverE bytes.
+Parameter recv : connection_id -> nat -> ServerM bytes.
 
 (* Receive a bytestring of length (exactly) [n]. *)
-Parameter recv_full : connection_id -> nat -> M serverE bytes.
+Parameter recv_full : connection_id -> nat -> ServerM bytes.
 
 (* Send all bytes in a bytestring. *)
-Parameter send : connection_id -> bytes -> M serverE unit.
+Parameter send : connection_id -> bytes -> ServerM unit.
 
 End ServerIface.
 
 (** ** Observer *)
 
-(* Module to define specifications as "observers".
+(* Module to define specifications as "observer" ITrees.
    For more details, see [Lib.SimpleSpec_Observer]. *)
 Module Type ObserverIface.
 
-(* The interface of observer is similar to servers;
+(** The type of observations that can be made. *)
+(* The interface of observers is similar to servers;
    the difference is that observers only consume bytes,
    while servers can produce bytes with [send]. *)
-Parameter specE : Type -> Type.
+Inductive observerE : Type -> Type :=
+| (* Observe the creation of a new connection *)
+  ObsConnect : observerE connection_id
 
-(* Internal nondeterminism is implemented via [nondetE]. *)
-Declare Instance nondet_spec : nondetE -< specE.
+| (* Observe a byte going into the server on a particular
+     connection *)
+  ObsToServer : connection_id -> observerE byte
 
-(* Observe a new connection. *)
-Parameter obs_connect : M specE connection_id.
+  (* Observe a byte going out of the server. *)
+| ObsFromServer : connection_id -> observerE (option byte).
 
-(* Observe a byte sent to the server. *)
-Parameter obs_to_server : connection_id -> M specE byte.
+(* The [ObsFromServer] effect returns an [option].
+   [None] is a "hole" in the observed trace, it represents a
+   message hypothetically sent by the server and that we haven't
+   yet received. These holes allow us to keep exploring an
+   observer even in the presence of partial outputs from the
+   server. *)
 
-(* Observe a byte sent from the server. A [None] result is a
-   "hypothetical" byte of unknown value (a hole in the observed
-   trace), intuitively meaning that no more bytes have
-   been received from the server on this connection, but the
-   server could have sent some. *)
-Parameter obs_from_server : connection_id -> M specE (option byte).
+
+(* The observer monad we write specifications in. *)
+Definition ObserverM := M (failureE +' nondetE +' observerE).
+
+(* As usual, we provide some itree wrappers for these constructors. *)
+
+Definition obs_connect :
+  ObserverM connection_id := embed ObsConnect.
+Definition obs_to_server :
+  connection_id -> ObserverM byte := embed ObsToServer.
+Definition obs_from_server :
+  connection_id -> ObserverM (option byte) := embed ObsFromServer.
+
+(* Also some derived operations. *)
 
 (* Make an assertion on a value, if it exists. *)
+(* BCP: Think about how to explain this *)
 Parameter assert_on :
-  forall {A}, string -> option A -> (A -> bool) -> M specE unit.
+  forall {A}, string -> option A -> (A -> bool) -> ObserverM unit.
 
 (* Observe a message of fixed-length sent to the server. *)
-Parameter obs_msg_to_server : nat -> connection_id -> M specE bytes.
+Parameter obs_msg_to_server : nat -> connection_id -> ObserverM bytes.
 
 (* Observe a message of fixed length received from the server
    and match it with an expected value, failing if they are not
    equal. *)
-Parameter obs_msg_from_server : connection_id -> bytes -> M specE unit.
+Parameter obs_msg_from_server : connection_id -> bytes -> ObserverM unit.
 
-(* [obs_msg_from_server] is implemented in terms of [obs_from_server].
-   In particular, when [obs_from_server] returns [None], we assume
-   that the hole stands for the next expected byte. *)
+(* [obs_msg_from_server] is implemented in terms of [obs_from_server]
+   and [assert_on].  In particular, when [obs_from_server] returns
+   [None], we assume that the hole stands for the next expected
+   byte. *)
 
 End ObserverIface.
 
@@ -101,10 +134,9 @@ End ObserverIface.
 
 Module Type TracesIface.
 
-(* An event can be observed to happen on the network,
-   either from the server's or the client's point of view.
-   It is paremeterized by the type to represent the server's
-   output... *)
+(* An event can be observed to happen on the network, either from the
+   server's or the client's point of view.  It is paremeterized by the
+   type to represent the server's output... *)
 Inductive event (byte' : Type) :=
 | NewConnection : connection_id -> event byte'
 | ToServer : connection_id -> byte -> event byte'
@@ -117,9 +149,9 @@ Definition trace byte' := list (event byte').
 Definition real_event := event byte.
 Definition real_trace := list real_event.
 
-(* ... but it will also be useful for testing to insert hypothetical
-   bytes of unknown values in a trace, representing values that the
-   server may have output but which have not reached the client yet. *)
+(* ... but it is also useful for testing to insert hypothetical bytes
+   of unknown values in a trace, representing values that the server
+   may have output but which have not reached the client yet. *)
 Definition hypo_event := event (option byte).
 Definition hypo_trace := list hypo_event.
 
@@ -127,38 +159,42 @@ Parameter real_to_hypo : real_trace -> hypo_trace.
 
 (* [is_server_trace server tr] holds if [tr] is a trace of
    the [server].  *)
-Parameter is_server_trace : itree_server -> real_trace -> Prop.
+Parameter is_server_trace : ServerM unit -> real_trace -> Prop.
 
-(* [is_spec_trace spec tr] holds if [tr] is a trace of the [spec]. *)
-Parameter is_spec_trace : itree_spec -> hypo_trace -> Prop.
+(* [is_observer_trace observer tr] holds if [tr] is a trace of
+   the [observer]. *)
+Parameter is_observer_trace : ObserverM unit -> hypo_trace -> Prop.
 
 (* Corresponding "server-side" and "client-side" traces. *)
-Parameter network_scrambled0 : real_trace -> real_trace -> Prop.
+Parameter network_scrambled : real_trace -> real_trace -> Prop.
 
 (* Property that a real trace [tr] is a scrambled trace of some
    spec trace. *)
-Definition is_scrambled_trace : itree_spec -> real_trace -> Prop :=
-  fun spec tr =>
+Definition is_scrambled_trace : ObserverM unit -> real_trace -> Prop :=
+  fun observer tr =>
     exists str,
-      network_scrambled0 str tr /\
-      is_spec_trace spec (real_to_hypo str).
+      network_scrambled str tr /\
+      is_observer_trace observer (real_to_hypo str).
 
-(* A server ([server : itree_server]) refines a "linear spec"
-   ([spec : itree_spec]) if, for every trace [tr] that the
+(* A server ([server : ServerM unit]) refines a "linear spec"
+   ([observer : ObserverM unit]) if, for every trace [tr] that the
    server can produce, and every trace [str] that can be observed
-   from it via the network, it can be explained by a
-   "descrambled trace" [dstr] in the "linear spec".  *)
-Parameter refines_mod_network : itree_server -> itree_spec -> Prop.
-
-(* BCP: Proposal: Define ServerM := M (nondetE +' serverE) and
-   ObserverM := M (nondetE +' observerE), where observerE = current
-   specE.  Then replace itree_server with ServerM unit, etc.. *)
+   from it via the network, it can be explained by a "descrambled
+   trace" [dstr] in the "linear spec".
+   Some examples can be found in [Spec/Swap_ExampleServers.v].
+ *)
+Parameter refines_mod_network :
+  ObserverM unit -> ServerM unit -> Prop.
 
 (* Tests *)
 
-(* A test for [is_spec_trace]. *)
-Parameter is_spec_trace_test :
-  nat -> itree_spec -> hypo_trace -> simple_result.
+(* See [Lib.Util.result] for the definition of the test result
+   types below. *)
+
+(* A test for [is_observer_trace]. *)
+(* TODO: reuse comment above the definition of this thing? *)
+Parameter is_observer_trace_test :
+  nat -> ObserverM unit -> hypo_trace -> simple_result.
 
 (* Test result of descrambling: if a descrambling is found,
    it gets returned. *)
@@ -166,76 +202,12 @@ Definition descrambled_result := result hypo_trace unit.
 
 (* A test for [is_scrambled_trace]. *)
 Parameter is_scrambled_trace_test :
-  nat -> itree_spec -> real_trace -> descrambled_result.
+  nat -> ObserverM unit -> real_trace -> descrambled_result.
 
-(* Check that every trace of the server can be descrambled into
+(* A test for [refines_mod_network].
+   Check that every trace of the server can be descrambled into
    a trace of the spec. *)
 Parameter refines_mod_network_test :
-  M specE unit -> M serverE unit -> Checker.
+  ObserverM unit -> ServerM unit -> Checker.
 
 End TracesIface.
-
-(** * Implementations *)
-
-Module Observer <: ObserverIface.
-Import Lib.SimpleSpec_Observer.
-Definition specE := specE.
-Instance nondet_spec : nondetE -< specE.
-Proof. typeclasses eauto. Defined.
-Definition obs_connect := @obs_connect specE _.
-Definition obs_to_server := @obs_to_server specE _.
-Definition obs_from_server := @obs_from_server specE _.
-Definition assert_on A := @assert_on specE A _.
-Definition obs_msg_to_server := @obs_msg_to_server specE _.
-Definition obs_msg_from_server := @obs_msg_from_server specE _ _.
-End Observer.
-
-Module Network : ServerIface.
-Definition serverE := Network.serverE.
-Instance networkE_server : networkE -< serverE.
-Proof. typeclasses eauto. Defined.
-Instance nondet_server : nondetE -< serverE.
-Proof. typeclasses eauto. Defined.
-Definition accept := @Network.accept _ _.
-Definition recv_byte := @Network.recv_byte _ _.
-Definition send_byte := @Network.send_byte _ _.
-Definition recv := @Network.recv _ _ _.
-Definition recv_full := @Network.recv_full _ networkE_server.
-Definition send := @Network.send _ networkE_server.
-End Network.
-
-Module Traces : TracesIface.
-
-  Include SimpleSpec_Traces.
-
-  Definition real_to_hypo := real_to_hypo_trace.
-  Definition is_server_trace := Network.is_server_trace.
-  Definition is_spec_trace := SimpleSpec_Observer.is_spec_trace.
-
-  (* TODO: reuse comment above the definition of this thing? *)
-  Definition is_spec_trace_test := SimpleSpec_Observer.is_spec_trace_test.
-  
-  (* Property that a real trace [tr] is a scrambled trace of some
-   spec trace. *)
-  Definition is_scrambled_trace : itree_spec -> real_trace -> Prop :=
-    fun spec tr =>
-      exists str,
-        network_scrambled0 str tr /\
-        is_spec_trace spec (real_to_hypo str).
-
-  Definition descrambled_result := result hypo_trace unit.
-
-  (* Parameter is_spec_trace_of : nat -> itree_spec -> hypo_trace -> result. *)
-
-  Definition is_scrambled_trace_test :=
-    SimpleSpec_Descramble.is_scrambled_trace_of.
-
-  Definition refines_mod_network_test
-    := SimpleSpec_ServerTrace.refines_mod_network_test.
-  
-  Definition refines_mod_network
-    := SimpleSpec_Refinement.ScramblingRefinement.refines_mod_network.
-  
-End Traces.
-
-  
