dw/DeepWeb/Lib/SanityCheck.v
@@ -1,0 +1,72 @@
+(* Check that the interfaces defined in [Lib.SimpleSpec]
+   are actually implemented by the modules actually
+   exported by [Lib.SimpleSpec]. *)
+
+Require Import DeepWeb.Free.Monad.Free.
+Require Import DeepWeb.Free.Monad.Common.
+Import SumNotations.
+
+Require Import DeepWeb.Lib.Util.
+
+From DeepWeb Require Import
+     Lib.SimpleSpec_Server
+     Lib.SimpleSpec_Observer
+     Lib.SimpleSpec_Descramble
+     Lib.SimpleSpec_Traces
+     Lib.SimpleSpec_Refinement
+     Lib.SimpleSpec_ServerTrace
+     Lib.SimpleSpec_NetworkModel
+     Lib.SimpleSpec.
+
+Module Network <: ServerIface.
+Include Lib.SimpleSpec_Server.ServerType.
+Definition E := failureE +' nondetE +' serverE.
+Definition ServerM := M E.
+Definition accept := @accept E _.
+Definition recv_byte := @recv_byte E _.
+Definition send_byte := @send_byte E _.
+Definition recv := @recv E _ _.
+Definition recv_full := @recv_full E _.
+Definition send := @send E _.
+End Network.
+
+Module Observer <: ObserverIface.
+Include Lib.SimpleSpec_Observer.ObserverType.
+Definition E := failureE +' nondetE +' observerE.
+Definition ObserverM := ObserverM.
+Definition obs_connect := @obs_connect E _.
+Definition obs_to_server := @obs_to_server E _.
+Definition obs_from_server := @obs_from_server E _.
+Definition assert_on A := @assert_on E A _ _.
+Definition obs_msg_to_server := @obs_msg_to_server E _.
+Definition obs_msg_from_server := @obs_msg_from_server E _ _ _.
+End Observer.
+
+Module Traces : TracesIface.
+
+  Include SimpleSpec_Traces.
+
+  Definition real_to_hypo := real_to_hypo_trace.
+  Definition is_server_trace := SimpleSpec_Server.is_server_trace.
+  Definition is_observer_trace := SimpleSpec_Observer.is_observer_trace.
+  Definition is_observer_trace_test := SimpleSpec_Observer.is_observer_trace_test.
+  (* Property that a real trace [tr] is a scrambled trace of some
+   spec trace. *)
+  Definition is_scrambled_trace : ObserverM unit -> real_trace -> Prop :=
+    fun observer tr =>
+      exists str,
+        network_scrambled str tr /\
+        is_observer_trace observer (real_to_hypo str).
+
+  Definition descrambled_result := Lib.Util.result hypo_trace unit.
+
+  Definition is_scrambled_trace_test :=
+    SimpleSpec_Descramble.is_scrambled_trace_test.
+
+  Definition refines_mod_network_test
+    := SimpleSpec_ServerTrace.refines_mod_network_test.
+
+  Definition refines_mod_network
+    := SimpleSpec_Refinement.refines_mod_network.
+
+End Traces.
