dw/DeepWeb/Lib/SimpleSpec_Refinement.v
@@ -8,7 +8,6 @@ From Custom Require Map.
 
 Require Import DeepWeb.Free.Monad.Free.
 Require Import DeepWeb.Free.Monad.Common.
-Import NonDeterminismBis.
 Import SumNotations.
 
 Require Import DeepWeb.Lib.Util.
@@ -20,6 +19,8 @@ From DeepWeb Require Import
      Lib.SimpleSpec_Scramble
      Lib.SimpleSpec_Traces.
 
+Import SimpleSpec_Scramble.ScramblingFacts.
+
 Set Bullet Behavior "Strict Subproofs".
 
 (* The definition of "refinement" between an itree representing
@@ -27,36 +28,35 @@ Set Bullet Behavior "Strict Subproofs".
    as a specification. The [ScramblingFacts] that the
    theorems below depend on are defined and proved in
    [Lib/SimpleSpec_Scramble.v]. *)
-Module MkScramblingRefinement (ScramblingFacts : ScramblingTypes).
 
-Import ScramblingFacts.
-
-(* A server ([server : itree_server]) refines a "linear spec"
-   ([spec : itree_spec]) if, for every trace [tr] that the
+(* A server ([server : ServerM unit]) refines a "linear spec"
+   ([observer : ObserverM unit]) if, for every trace [tr] that the
    server can produce, and every trace [str] that can be observed
-   from it via the network, it can be explained by a
-   "descrambled trace" [dstr] in the "linear spec".  *)
-Definition refines_mod_network server spec : Prop :=
+   from it via the network, it can be explained by a "descrambled
+   trace" [dstr] in the "linear spec".
+   Some examples can be found in [Spec/Swap_ExampleServers.v].
+ *)
+Definition refines_mod_network observer server : Prop :=
   forall tr : real_trace,
     is_server_trace server tr ->
     forall str : real_trace,
-      network_scrambled0 tr str ->
+      network_scrambled tr str ->
       exists dstr : real_trace,
-        network_scrambled0 dstr str /\
-        is_spec_trace spec dstr.
+        network_scrambled dstr str /\
+        is_observer_trace observer dstr.
 
 (* It turns out that we can simplify this property
    (three quantifiers!) to remove an intermediate step.
    We can directly descramble only the traces of the server.
    [strong_sound] and [strong_complete] shown below establish
    the equivalence between these two properties. *)
-Definition strong_refines_mod_network server spec : Prop :=
+Definition strong_refines_mod_network observer server : Prop :=
   forall tr : real_trace,
     wf_trace tr ->
     is_server_trace server tr ->
       exists dstr : real_trace,
-        network_scrambled0 dstr tr /\
-        is_spec_trace spec dstr.
+        network_scrambled dstr tr /\
+        is_observer_trace observer dstr.
 
 (* [strong_sound] and [strong_complete] rely on two properties
    of the [network_scrambled] relation: it is reflexive
@@ -90,11 +90,6 @@ Proof.
   exists dstr.
   auto.
 Qed.
-
-End MkScramblingRefinement.
-
-Module Export ScramblingRefinement :=
-  MkScramblingRefinement ScramblingFacts.
 
 (* [refines_mod_network] is part of the toplevel property
    about the swap server, stated in [Spec/TopLevelSpec.v]. *)
