dw/DeepWeb/Test/TestInternal.v
@@ -1,0 +1,36 @@
+(*! Section CLikeTest *)(*! extends BaseTest *)
+
+(* Simulate a server (defined in Coq, hence "internal"),
+   nondeterministically returning the new state of the network. *)
+
+Typeclasses eauto := 6.
+
+From QuickChick Require Import QuickChick.
+From ExtLib Require Monad.
+
+From DeepWeb Require Import
+     Lib.SimpleSpec.
+
+From DeepWeb.Spec Require
+     Swap_CLikeSpec
+     Swap_SimpleSpec.
+
+Definition swap_server : ServerM unit :=
+  Swap_CLikeSpec.test_server.
+Definition swap_observer : ObserverM unit :=
+  Swap_SimpleSpec.swap_observer_def.
+
+(* Enumerate the traces of the [server'] itree (swap server). *)
+Definition random_trace_server :=
+  random_trace 500 10 swap_server.
+
+(*
+Sample random_trace_server.
+*)
+
+Definition test :=
+  refines_mod_network_test
+    Swap_SimpleSpec.swap_observer_def
+    swap_server.
+
+(*! QuickChick test. *)
